src/ssa/extraction/llvmcaml.ml
@@ -10,18 +10,39 @@ let coqcond_2_llvmicmp (c:cond) : Llvm.Icmp.t = Coq2llvm.translate_icond c
 
 module TargetData = struct
 
-  let getTypeAllocSize (td:LLVMsyntax.layouts) t = 
-    let ltd = Llvm_target.TargetData.create (coqtd_2_llvmtd td) in
-    let sz = Int64.to_int (Llvm_target.get_type_alloc_size ltd (coqtype_2_llvmtype t)) in
-    Llvm_target.TargetData.dispose ltd;
-    Some sz
+  type t = ExecutionEngine.t * Llvm.llmodule
+
+  let getTypeAllocSize (td:t) typ = 
+    let (ee, _) = td in
+    let ltd = ExecutionEngine.target_data ee in
+    Some (Int64.to_int (Llvm_target.get_type_alloc_size ltd (coqtype_2_llvmtype typ)))
 		
   let getTypeAllocSizeInBits x y = failwith "undef"
   let _getStructElementOffset x y z = failwith "undef"
   let getStructElementOffset x y z = failwith "undef"
   let getStructElementOffsetInBits x y z = failwith "undef"
   let _getStructElementContainingOffset x y z = failwith "undef"
-  let getStructElementContainingOffset x y z = failwith "undef"		
+  let getStructElementContainingOffset x y z = failwith "undef"
+  let _getIntAlignmentInfo x = failwith "undef"
+  let getIntAlignmentInfo x = failwith "undef"
+  let _getPointerAlignmentInfo x = failwith "undef"
+  let getPointerAlignmentInfo x = failwith "undef"
+  let _getStructAlignmentInfo x = failwith "undef"
+  let getStructAlignmentInfo x = failwith "undef"
+  let _getPointerSize x = failwith "undef"
+  let getPointerSize x = failwith "undef"
+  let getPointerSizeInBits x = failwith "undef"
+  let getTypeSizeInBits_and_Alignment x = failwith "undef"
+  let getListTypeSizeInBits_and_Alignment x = failwith "undef"
+  let getAlignment x = failwith "undef"
+  let getABITypeAlignment x = failwith "undef"
+  let getPrefTypeAlignment x = failwith "undef"
+  let getTypeSizeInBits x = failwith "undef"
+  let getTypeStoreSize x = failwith "undef"
+  let getTypeStoreSizeInBits x = failwith "undef"
+  let getStructSizeInBytes x = failwith "undef"
+  let getStructSizeInBits x = failwith "undef"
+  let getStructAlignment x = failwith "undef"					
 		
 end	
 
@@ -43,23 +64,21 @@ module GenericValue = struct
   let _list_const_struct2GV x y z = failwith "_list_const_struct2GV undef" 
 
   (* used at runtime *)
-  let blk2gv (td:LLVMsyntax.layouts) (v:t) = v
+  let blk2gv (td:TargetData.t) (v:t) = v
 
-  let isZero (td:LLVMsyntax.layouts) (v:t) = GenericValue.as_int v == 0
+  let isZero (td:TargetData.t) (v:t) = GenericValue.as_int v == 0
 
-  let const2GV (td:LLVMsyntax.layouts) gl (c:const) : t option = 
+  let const2GV (td:TargetData.t) gl (c:const) : t option = 
     let ctx = Llvm.global_context() in
-    let ltd = Llvm_target.TargetData.create (coqtd_2_llvmtd td) in
-		let og =
-    (match c with
+    let (ee, _) = td in
+    let ltd = ExecutionEngine.target_data ee in
+    match c with
     | Coq_const_int (sz, i) -> Some (GenericValue.of_constant ltd (Coq2llvm.translate_constant ctx c))
     | Coq_const_undef t -> Some (GenericValue.of_constant ltd (Coq2llvm.translate_constant ctx c)) 
     | Coq_const_null t -> Some (GenericValue.of_constant ltd (Coq2llvm.translate_constant ctx c)) 
     | Coq_const_arr cs -> Some (GenericValue.of_constant ltd (Coq2llvm.translate_constant ctx c))  
     | Coq_const_struct cs -> Some (GenericValue.of_constant ltd (Coq2llvm.translate_constant ctx c))
-    | Coq_const_gid (_,id) -> Assoclist.lookupAL gl id) in
-		Llvm_target.TargetData.dispose ltd;
-		og
+    | Coq_const_gid (_,id) -> Assoclist.lookupAL gl id
 
   let mgep x y z w = failwith "mgep undef"
 
@@ -67,13 +86,13 @@ module GenericValue = struct
 
   let insertGenericValue x y z a b = failwith "extractGenericValue undef"
 
-  let mbop (td:LLVMsyntax.layouts) (op:LLVMsyntax.bop) (bsz:LLVMsyntax.sz) (gv1:t) (gv2:t) = 
+  let mbop (td:TargetData.t) (op:LLVMsyntax.bop) (bsz:LLVMsyntax.sz) (gv1:t) (gv2:t) = 
     let gv = (GenericValue.binary_op gv1 gv2 (Llvm.integer_type (Llvm.global_context()) bsz) (coqbop_2_llvmopcode op)) in
     eprintf "  Mbop s=%d gv1=%s gv2=%s r=%s\n" bsz 
 		  (GenericValue.to_string gv1) (GenericValue.to_string gv2) (GenericValue.to_string gv);flush_all();
 		Some gv
 
-  let mcast (td:LLVMsyntax.layouts) (op:LLVMsyntax.castop) (t1:LLVMsyntax.typ) (gv1:t) (t2:LLVMsyntax.typ) =
+  let mcast (td:TargetData.t) (op:LLVMsyntax.castop) (t1:LLVMsyntax.typ) (gv1:t) (t2:LLVMsyntax.typ) =
     let gv =
     (match op with
     | Coq_castop_fptoui -> GenericValue.fptoui gv1 (coqtype_2_llvmtype t1) (coqtype_2_llvmtype t2)
@@ -81,11 +100,9 @@ module GenericValue = struct
     | Coq_castop_uitofp -> GenericValue.uitofp gv1 (coqtype_2_llvmtype t2)
     | Coq_castop_sitofp -> GenericValue.sitofp gv1 (coqtype_2_llvmtype t2)
     | Coq_castop_ptrtoint -> GenericValue.ptrtoint gv1 (coqtype_2_llvmtype t1) (coqtype_2_llvmtype t2)
-    | Coq_castop_inttoptr -> 
-			  let ltd = Llvm_target.TargetData.create (coqtd_2_llvmtd td) in
-				let gv2 = GenericValue.inttoptr ltd gv1 (coqtype_2_llvmtype t2) in
-				Llvm_target.TargetData.dispose ltd;
-				gv2
+    | Coq_castop_inttoptr -> let (ee, _) = td in
+                             let ltd = ExecutionEngine.target_data ee in
+			                       GenericValue.inttoptr ltd gv1 (coqtype_2_llvmtype t2)
     | Coq_castop_bitcast -> GenericValue.bitcast gv1 
                               (coqtype_2_llvmtype t1) 
                               (Llvm.global_context()) 
@@ -95,7 +112,7 @@ module GenericValue = struct
 		  (GenericValue.to_string gv1) (GenericValue.to_string gv);flush_all();
 	  Some gv
 
-  let mext (td:layouts) (op:extop) (t1:typ) (gv1:t) (t2:typ) =
+  let mext (td:TargetData.t) (op:extop) (t1:typ) (gv1:t) (t2:typ) =
     let gv =
     (match op with
     | Coq_extop_z -> GenericValue.zext gv1 (coqtype_2_llvmtype t2)
@@ -105,7 +122,7 @@ module GenericValue = struct
 		  (GenericValue.to_string gv1) (GenericValue.to_string gv);flush_all();
 	  Some gv
 
-  let micmp (td:layouts) (c:cond) (t:typ) (gv1:t) (gv2:t) =
+  let micmp (td:TargetData.t) (c:cond) (t:typ) (gv1:t) (gv2:t) =
     let gv = GenericValue.icmp gv1 gv2 (coqtype_2_llvmtype t) (coqcond_2_llvmicmp c) in
     eprintf "  Micmp t=%s gv1=%s gv2=%s r=%s\n" (Coq_pretty_printer.string_of_typ t)
 		  (GenericValue.to_string gv1) (GenericValue.to_string gv2) (GenericValue.to_string gv);flush_all();
@@ -122,7 +139,7 @@ module Mem = struct
 
   (* let initmem = failwith "initmem undef" *)
 
-  let malloc (td:LLVMsyntax.layouts) m size (a:LLVMsyntax.align) = 
+  let malloc (td:TargetData.t) m size (a:LLVMsyntax.align) = 
     let (ee, _) = m in
     match (ExecutionEngine.malloc_memory size ee) with
     | Some gv -> 
@@ -132,33 +149,33 @@ module Mem = struct
     		eprintf "  Malloc None";flush_all();
 			  None
 
-  let free (td:LLVMsyntax.layouts) m ptr =
+  let free (td:TargetData.t) m ptr =
     let (ee, _) = m in
     let _ = ExecutionEngine.free_memory ptr ee in
     eprintf "  Mfree ptr=%s\n" (GenericValue.to_string ptr);flush_all();				
 		Some m
 
-  let mload (td:LLVMsyntax.layouts) m ptr t (a:LLVMsyntax.align) =
+  let mload (td:TargetData.t) m ptr t (a:LLVMsyntax.align) =
     let (ee, _) = m in
 		let gv = ExecutionEngine.load_value_from_memory ptr (coqtype_2_llvmtype t) ee in
 		eprintf "  Mload ptr=%s r=%s\n" (GenericValue.to_string ptr) (GenericValue.to_string gv);flush_all();
 		Some gv
 
-  let mstore (td:LLVMsyntax.layouts) m ptr t gv (a:LLVMsyntax.align) =
+  let mstore (td:TargetData.t) m ptr t gv (a:LLVMsyntax.align) =
 		eprintf "  Mstore ptr=%s v=%s\n" (GenericValue.to_string ptr) (GenericValue.to_string gv);flush_all();
 		let (ee, _) = m in
     let _ = ExecutionEngine.store_value_to_memory gv ptr (coqtype_2_llvmtype t) ee in
     Some m
 		
 	let getRealName (id:LLVMsyntax.id) =
-	if String.length id <= 1
-	then id
-	else 
-		if String.get id 0 = '@' or String.get id 0 = '%'
-		then String.sub id 1 (String.length id-1)
-		else id
+	  if String.length id <= 1
+	  then id
+	  else 
+	  	if String.get id 0 = '@' or String.get id 0 = '%'
+  		then String.sub id 1 (String.length id-1)
+  		else id
 
-  let initGlobal (td:LLVMsyntax.layouts) gl m (id0:LLVMsyntax.id) 
+  let initGlobal (td:TargetData.t) gl m (id0:LLVMsyntax.id) 
                  (t:LLVMsyntax.typ)(c:LLVMsyntax.const)(align0:LLVMsyntax.align) =
     let (ee, mm) = m in
     match Llvm.lookup_global (getRealName id0) mm with
@@ -167,6 +184,15 @@ module Mem = struct
        | Some gv -> Some (gv, m)
        | None -> None)
     | None -> None
+
+  let initTargetData (td:LLVMsyntax.layouts) (m:t) = m
+
+  let callExternalFunction m (fid:LLVMsyntax.id) (args:GenericValue.t list) = 
+		eprintf "  Mcall external fun=%s\n" fid;flush_all();
+		let (ee, mm) = m in
+    match Llvm.lookup_function (getRealName fid) mm with
+    | Some fv -> (Some (ExecutionEngine.call_external_function fv (Array.of_list args) ee), m)
+    | None -> failwith "callExternalFunction: cannot find function"
 		
 end
 
