src/ssa/extraction/ssa_main.ml
@@ -60,5 +60,3 @@ let () = match Sys.argv with
         | _ -> main "Input.bc"
 
 
-
-
